src/ConcurrentFS.v
@@ -1,243 +1,16 @@
 Require Import CCL.
 Require Import Hashmap.
-Require Import OptimisticTranslator OptimisticFS.
 
-Require AsyncFS.
-(* imports for DirTreeRep.rep *)
-Import Log FSLayout Inode.INODE BFile.
-
-(* various other imports *)
-Import BFILE.
-Import SuperBlock.
-Import GenSepN.
-Import Pred.
-
-Require Import HomeDirProtocol.
-Require Import RelationClasses.
+Require Import FSProtocol.
+Require Import OptimisticFS.
 Require Import ConcurCompile.
 
-Record FsParams :=
-  { cache: ident; (* : Cache *)
-    vdisk: ident; (* : Disk *)
-    fsmem: ident; (* : memsstate *)
-    fstree: ident; (* : dirtree *)
-    fshomedirs: ident; (* thread_homes *)
-    }.
+Import FSLayout Log BFile.
 
 Section ConcurrentFS.
 
-  Variable fsxp: fs_xparams.
   Variable P:FsParams.
-
-  Definition fs_rep vd hm mscs tree :=
-    exists ds ilist frees,
-      LOG.rep (FSLayout.FSXPLog fsxp) (SB.rep fsxp)
-              (LOG.NoTxn ds) (MSLL mscs) hm (add_buffers vd) /\
-      (DirTreeRep.rep fsxp Pred.emp tree ilist frees mscs)
-        (list2nmem (ds!!)).
-
-  Definition fs_invariant d hm tree (homedirs: thread_homes) : heappred :=
-    (fstree P |-> abs tree *
-     fshomedirs P |-> abs homedirs *
-     exists c vd mscs,
-       cache P |-> val c *
-       vdisk P |-> absMem vd *
-       [[ CacheRep d c vd ]] *
-       fsmem P |-> val mscs *
-       [[ fs_rep vd hm mscs tree ]])%pred.
-
-  Theorem fs_invariant_unfold : forall d hm tree homedirs h,
-      fs_invariant d hm tree homedirs h ->
-      exists c vd mscs,
-        (fstree P |-> abs tree * fshomedirs P |-> abs homedirs *
-         cache P |-> val c *
-         vdisk P |-> absMem vd *
-         fsmem P |-> val mscs)%pred h /\
-        CacheRep d c vd /\
-        fs_rep vd hm mscs tree.
-  Proof.
-    unfold fs_invariant; intros.
-    SepAuto.destruct_lifts.
-    descend; intuition eauto.
-  Qed.
-
-  Theorem fs_invariant_refold : forall tree homedirs d c vd hm mscs h,
-      (fstree P |-> abs tree * fshomedirs P |-> abs homedirs *
-       cache P |-> val c *
-       vdisk P |-> absMem vd *
-       fsmem P |-> val mscs)%pred h ->
-      CacheRep d c vd ->
-      fs_rep vd hm mscs tree ->
-      fs_invariant d hm tree homedirs h.
-  Proof.
-    unfold fs_invariant; intros.
-    SepAuto.pred_apply; SepAuto.cancel.
-  Qed.
-
-  Definition fs_guarantee tid (sigma sigma':Sigma) :=
-    exists tree tree' homedirs,
-      fs_invariant (Sigma.disk sigma) (Sigma.hm sigma) tree homedirs (Sigma.mem sigma) /\
-      fs_invariant (Sigma.disk sigma') (Sigma.hm sigma') tree' homedirs (Sigma.mem sigma') /\
-      homedir_guarantee tid homedirs tree tree' /\
-      Sigma.l sigma' = Sigma.l sigma.
-
-  Theorem fs_rely_same_fstree : forall tid sigma sigma' tree homedirs,
-      fs_invariant (Sigma.disk sigma) (Sigma.hm sigma) tree homedirs (Sigma.mem sigma) ->
-      fs_invariant (Sigma.disk sigma') (Sigma.hm sigma') tree homedirs (Sigma.mem sigma') ->
-      Sigma.l sigma' = Sigma.l sigma ->
-      Rely fs_guarantee tid sigma sigma'.
-  Proof.
-    intros.
-    constructor.
-    exists (S tid); intuition.
-    unfold fs_guarantee.
-    descend; intuition eauto.
-    reflexivity.
-  Qed.
-
-  Section InvariantUniqueness.
-
-    Ltac mem_eq m a v :=
-      match goal with
-      | [ H: context[ptsto a v] |- _ ] =>
-        let Hptsto := fresh in
-        assert ((exists F, F * a |-> v)%pred m) as Hptsto by
-              (SepAuto.pred_apply' H; SepAuto.cancel);
-        unfold exis in Hptsto; destruct Hptsto;
-        apply ptsto_valid' in Hptsto
-      end.
-
-    Lemma fs_invariant_tree_unique : forall d hm tree homedirs
-                                       d' hm' tree' homedirs' m,
-        fs_invariant d hm tree homedirs m ->
-        fs_invariant d' hm' tree' homedirs' m ->
-        tree = tree'.
-    Proof.
-      unfold fs_invariant; intros.
-      mem_eq m (fstree P) (abs tree).
-      mem_eq m (fstree P) (abs tree').
-      rewrite H1 in H2; inversion H2; inj_pair2.
-      auto.
-    Qed.
-
-    Lemma fs_invariant_homedirs_unique : forall d hm tree homedirs
-                                       d' hm' tree' homedirs' m,
-        fs_invariant d hm tree homedirs m ->
-        fs_invariant d' hm' tree' homedirs' m ->
-        homedirs = homedirs'.
-    Proof.
-      unfold fs_invariant; intros.
-      mem_eq m (fshomedirs P) (abs homedirs).
-      mem_eq m (fshomedirs P) (abs homedirs').
-      rewrite H1 in H2; inversion H2; inj_pair2.
-      auto.
-    Qed.
-
-  End InvariantUniqueness.
-
-  Ltac invariant_unique :=
-    repeat match goal with
-           | [ H: fs_invariant _ _ ?tree _ ?m,
-                  H': fs_invariant _ _ ?tree' _ ?m |- _ ] =>
-             first [ constr_eq tree tree'; fail 1 |
-                     assert (tree' = tree) by
-                         apply (fs_invariant_tree_unique H' H); subst ]
-           | [ H: fs_invariant _ _ _ ?homedirs ?m,
-                  H': fs_invariant _ _ _ ?homedirs' ?m |- _ ] =>
-             first [ constr_eq homedirs homedirs'; fail 1 |
-                     assert (homedirs' = homedirs) by
-                         apply (fs_invariant_homedirs_unique H' H); subst ]
-           end.
-
-  Theorem fs_rely_invariant : forall tid sigma sigma' tree homedirs,
-      fs_invariant (Sigma.disk sigma) (Sigma.hm sigma) tree homedirs (Sigma.mem sigma) ->
-      Rely fs_guarantee tid sigma sigma' ->
-      exists tree', fs_invariant (Sigma.disk sigma') (Sigma.hm sigma') tree' homedirs (Sigma.mem sigma').
-  Proof.
-    unfold fs_guarantee; intros.
-    generalize dependent tree.
-    induction H0; intros; repeat deex; eauto.
-    invariant_unique.
-    eauto.
-    edestruct IHclos_refl_trans1; eauto.
-  Qed.
-
-  Lemma fs_rely_invariant' : forall tid sigma sigma',
-      Rely fs_guarantee tid sigma sigma' ->
-      forall tree homedirs,
-        fs_invariant (Sigma.disk sigma) (Sigma.hm sigma) tree homedirs (Sigma.mem sigma) ->
-        exists tree',
-          fs_invariant (Sigma.disk sigma') (Sigma.hm sigma') tree' homedirs (Sigma.mem sigma').
-  Proof.
-    intros.
-    eapply fs_rely_invariant; eauto.
-  Qed.
-
-  Theorem fs_homedir_rely : forall tid sigma sigma' tree homedirs tree',
-      fs_invariant (Sigma.disk sigma) (Sigma.hm sigma) tree homedirs (Sigma.mem sigma) ->
-      Rely fs_guarantee tid sigma sigma' ->
-      fs_invariant (Sigma.disk sigma') (Sigma.hm sigma') tree' homedirs (Sigma.mem sigma') ->
-      homedir_rely tid homedirs tree tree'.
-  Proof.
-    unfold fs_guarantee; intros.
-    generalize dependent tree'.
-    generalize dependent tree.
-    apply Operators_Properties.clos_rt_rt1n in H0.
-    induction H0; intros; repeat deex; invariant_unique.
-    - reflexivity.
-    - match goal with
-      | [ H: homedir_guarantee _ _ _ _ |- _ ] =>
-        specialize (H _ ltac:(eauto))
-      end.
-      specialize (IHclos_refl_trans_1n _ ltac:(eauto) _ ltac:(eauto)).
-      unfold homedir_rely in *; congruence.
-  Qed.
-
-  Theorem fs_lock_rely : forall tid sigma sigma',
-      Rely fs_guarantee tid sigma sigma' ->
-      Sigma.l sigma' = Sigma.l sigma.
-  Proof.
-    unfold fs_guarantee; intros.
-    apply Operators_Properties.clos_rt_rt1n in H.
-    induction H; intros; repeat deex; congruence.
-  Qed.
-
-  Lemma fs_rely_preserves_subtree : forall tid sigma sigma' tree homedirs tree' path f,
-      find_subtree (homedirs tid ++ path) tree = Some f ->
-      fs_invariant (Sigma.disk sigma) (Sigma.hm sigma) tree homedirs (Sigma.mem sigma) ->
-      Rely fs_guarantee tid sigma sigma' ->
-      fs_invariant (Sigma.disk sigma') (Sigma.hm sigma') tree' homedirs (Sigma.mem sigma') ->
-      find_subtree (homedirs tid ++ path) tree' = Some f.
-  Proof.
-    intros.
-    eapply fs_homedir_rely in H1; eauto.
-    unfold homedir_rely in H1.
-    eapply find_subtree_app' in H; repeat deex.
-    erewrite find_subtree_app; eauto.
-    congruence.
-  Qed.
-
-  Theorem fs_guarantee_refl : forall tid sigma homedirs,
-      (exists tree, fs_invariant (Sigma.disk sigma) (Sigma.hm sigma) tree homedirs (Sigma.mem sigma)) ->
-      fs_guarantee tid sigma sigma.
-  Proof.
-    intros; deex.
-    unfold fs_guarantee; descend; intuition eauto.
-    reflexivity.
-  Qed.
-
-  Theorem fs_guarantee_trans : forall tid sigma sigma' sigma'',
-      fs_guarantee tid sigma sigma' ->
-      fs_guarantee tid sigma' sigma'' ->
-      fs_guarantee tid sigma sigma''.
-  Proof.
-    unfold fs_guarantee; intuition.
-    repeat deex; invariant_unique.
-
-    descend; intuition eauto.
-    etransitivity; eauto.
-    congruence.
-  Qed.
+  Definition G := fs_guarantee P.
 
   Inductive SyscallResult {T} :=
   | Done (v:T)
@@ -340,7 +113,7 @@ Section ConcurrentFS.
       {| precondition :=
            F (Sigma.mem sigma) /\
            CacheRep d c vd /\
-           fs_rep vd (Sigma.hm sigma) mscs tree /\
+           fs_rep P vd (Sigma.hm sigma) mscs tree /\
            fs_pre (fsspec a) tree /\
            Sigma.l sigma = l;
          postcondition :=
@@ -351,10 +124,10 @@ Section ConcurrentFS.
                match r with
                | Success _ (mscs', r) =>
                  fs_post (fsspec a) r /\
-                 fs_rep vd' (Sigma.hm sigma') mscs' (fs_dirup (fsspec a) tree)
+                 fs_rep P vd' (Sigma.hm sigma') mscs' (fs_dirup (fsspec a) tree)
                | Failure e =>
                  (l = WriteLock -> e <> WriteRequired) /\
-                 fs_rep vd (Sigma.hm sigma') mscs tree
+                 fs_rep P vd (Sigma.hm sigma') mscs tree
                end /\
                hashmap_le (Sigma.hm sigma) (Sigma.hm sigma') ; |}.
 
@@ -366,17 +139,17 @@ Section ConcurrentFS.
   Lemma precondition_stable_rely_fwd : forall A T (spec: FsSpec A T) tid a
                                      sigma tree homedirs sigma',
       precondition_stable spec homedirs tid ->
-      fs_invariant (Sigma.disk sigma) (Sigma.hm sigma) tree homedirs (Sigma.mem sigma) ->
-      Rely fs_guarantee tid sigma sigma' ->
+      fs_invariant P (Sigma.disk sigma) (Sigma.hm sigma) tree homedirs (Sigma.mem sigma) ->
+      Rely G tid sigma sigma' ->
       fs_pre (spec a) tree ->
       exists tree',
-        fs_invariant (Sigma.disk sigma') (Sigma.hm sigma') tree' homedirs (Sigma.mem sigma') /\
+        fs_invariant P (Sigma.disk sigma') (Sigma.hm sigma') tree' homedirs (Sigma.mem sigma') /\
         homedir_rely tid homedirs tree tree' /\
         fs_pre (spec a) tree'.
   Proof.
     unfold precondition_stable; intros.
     match goal with
-    | [ H: fs_invariant _ _ _ _ _,
+    | [ H: fs_invariant _ _ _ _ _ _,
            H': Rely _ _ _ _ |- _ ] =>
       pose proof (fs_rely_invariant H H')
     end; deex.
@@ -387,15 +160,15 @@ Section ConcurrentFS.
     Spec _ (SyscallResult T) :=
     fun '(tree, homedirs, a) sigma =>
       {| precondition :=
-           (fs_invariant (Sigma.disk sigma) (Sigma.hm sigma) tree homedirs) (Sigma.mem sigma) /\
+           (fs_invariant P (Sigma.disk sigma) (Sigma.hm sigma) tree homedirs) (Sigma.mem sigma) /\
            Sigma.l sigma = Free /\
            fs_pre (fsspec a) tree /\
            precondition_stable fsspec homedirs tid;
          postcondition :=
            fun sigma' r =>
              exists tree',
-               (fs_invariant (Sigma.disk sigma') (Sigma.hm sigma') tree' homedirs) (Sigma.mem sigma') /\
-               Rely fs_guarantee tid sigma sigma' /\
+               (fs_invariant P (Sigma.disk sigma') (Sigma.hm sigma') tree' homedirs) (Sigma.mem sigma') /\
+               Rely G tid sigma sigma' /\
                homedir_rely tid homedirs tree tree' /\
                Sigma.l sigma' = Free /\
                match r with
@@ -405,9 +178,9 @@ Section ConcurrentFS.
                end |}.
 
   Lemma fs_rep_hashmap_incr : forall vd tree mscs hm hm',
-      fs_rep vd hm mscs tree ->
+      fs_rep P vd hm mscs tree ->
       hashmap_le hm hm' ->
-      fs_rep vd hm' mscs tree.
+      fs_rep P vd hm' mscs tree.
   Proof.
     unfold fs_rep; intros.
     repeat deex.
@@ -418,21 +191,21 @@ Section ConcurrentFS.
   Hint Resolve fs_rep_hashmap_incr.
 
   Definition readCacheMem_ok : forall tid,
-      cprog_spec fs_guarantee tid
+      cprog_spec G tid
                  (fun '(tree, homedirs) sigma =>
                     {| precondition :=
-                         fs_invariant (Sigma.disk sigma) (Sigma.hm sigma) tree homedirs (Sigma.mem sigma) /\
+                         fs_invariant P (Sigma.disk sigma) (Sigma.hm sigma) tree homedirs (Sigma.mem sigma) /\
                          Sigma.l sigma = Free;
                        postcondition :=
                          fun sigma' '(c, mscs) =>
                            exists tree',
-                             fs_invariant (Sigma.disk sigma') (Sigma.hm sigma') tree' homedirs (Sigma.mem sigma') /\
+                             fs_invariant P (Sigma.disk sigma') (Sigma.hm sigma') tree' homedirs (Sigma.mem sigma') /\
                              hashmap_le (Sigma.hm sigma) (Sigma.hm sigma') /\
-                             Rely fs_guarantee tid sigma sigma' /\
+                             Rely G tid sigma sigma' /\
                              homedir_rely tid homedirs tree tree' /\
                              (* mscs and c come from fs_invariant on sigma *)
                              (exists vd, CacheRep (Sigma.disk sigma) c vd /\
-                                   fs_rep vd (Sigma.hm sigma') mscs tree) /\
+                                    fs_rep P vd (Sigma.hm sigma') mscs tree) /\
                              Sigma.l sigma' = Sigma.l sigma |})
                  readCacheMem.
   Proof.
@@ -440,7 +213,7 @@ Section ConcurrentFS.
     step.
     destruct a as (tree & homedirs); simpl in *; intuition.
     match goal with
-    | [ H: fs_invariant _ _ _ _ _ |- _ ] =>
+    | [ H: fs_invariant _ _ _ _ _ _ |- _ ] =>
       pose proof (fs_invariant_unfold H); repeat deex
     end.
     descend; simpl in *; intuition eauto.
@@ -466,10 +239,10 @@ Section ConcurrentFS.
   Hint Resolve CacheRep_disk_eq.
 
   Theorem readonly_syscall_ok : forall T (p: OptimisticProg T) A (fsspec: FsSpec A T) tid,
-      (forall mscs c, cprog_spec fs_guarantee tid
-                          (fs_spec fsspec mscs Free c)
-                          (p mscs Free c)) ->
-      cprog_spec fs_guarantee tid
+      (forall mscs c, cprog_spec G tid
+                            (fs_spec fsspec mscs Free c)
+                            (p mscs Free c)) ->
+      cprog_spec G tid
                  (readonly_spec fsspec tid) (readonly_syscall p).
   Proof.
     unfold readonly_syscall, readonly_spec; intros.
@@ -483,7 +256,7 @@ Section ConcurrentFS.
     monad_simpl.
     eapply cprog_ok_weaken; [ eapply H | ]; simplify.
     match goal with
-    | [ H: fs_invariant _ _ _ _ _ |- _ ] =>
+    | [ H: fs_invariant _ _ _ _ _ _ |- _ ] =>
       pose proof (fs_invariant_unfold H); repeat deex
     end.
     descend; simpl in *; (intuition eauto); try congruence.
@@ -500,7 +273,7 @@ Section ConcurrentFS.
   Qed.
 
   Definition file_get_attr inum :=
-    retry_syscall (fun mscs => file_get_attr fsxp inum mscs)
+    retry_syscall (fun mscs => file_get_attr (fsxp P) inum mscs)
                   (fun tree => tree).
 
   Lemma exists_tuple : forall A B P,
@@ -523,18 +296,16 @@ Section ConcurrentFS.
            end.
 
   Theorem opt_file_get_attr_ok : forall inum mscs l tid c,
-      cprog_spec fs_guarantee tid
+      cprog_spec G tid
                  (fs_spec (fun '(pathname, f) =>
                              {| fs_pre :=
                                   fun tree => find_subtree pathname tree = Some (TreeFile inum f);
                                 fs_post :=
                                   fun '(r, _) => r = BFILE.BFAttr f;
                                 fs_dirup := fun tree => tree |}) mscs l c)
-                 (OptFS.file_get_attr fsxp inum mscs l c).
+                 (OptFS.file_get_attr (fsxp P) inum mscs l c).
   Proof.
   Admitted.
-
-  Hint Extern 0 {{ OptFS.file_get_attr _ _ _ _ _; _ }} => apply opt_file_get_attr_ok : prog.
 
   Lemma and_copy : forall (P Q:Prop),
       P ->
@@ -547,77 +318,77 @@ Section ConcurrentFS.
   (* translate remaining system calls for extraction *)
 
   Definition lookup dnum names :=
-    retry_syscall (fun mscs => lookup fsxp dnum names mscs)
+    retry_syscall (fun mscs => lookup (fsxp P) dnum names mscs)
                   (fun tree => tree).
 
   Definition read_fblock inum off :=
-    retry_syscall (fun mscs => OptFS.read_fblock fsxp inum off mscs)
+    retry_syscall (fun mscs => OptFS.read_fblock (fsxp P) inum off mscs)
                   (fun tree => tree).
 
   Definition file_set_attr inum attr :=
-    retry_syscall (fun mscs => OptFS.file_set_attr fsxp inum attr mscs)
+    retry_syscall (fun mscs => OptFS.file_set_attr (fsxp P) inum attr mscs)
                   (fun tree => tree).
 
   Definition file_truncate inum sz :=
-    retry_syscall (fun mscs => OptFS.file_truncate fsxp inum sz mscs)
+    retry_syscall (fun mscs => OptFS.file_truncate (fsxp P) inum sz mscs)
                   (fun tree => tree).
 
   Definition update_fblock_d inum off b :=
-    retry_syscall (fun mscs => OptFS.update_fblock_d fsxp inum off b mscs)
+    retry_syscall (fun mscs => OptFS.update_fblock_d (fsxp P) inum off b mscs)
                   (fun tree => tree).
 
   Definition create dnum name :=
-    retry_syscall (fun mscs => OptFS.create fsxp dnum name mscs)
+    retry_syscall (fun mscs => OptFS.create (fsxp P) dnum name mscs)
                   (fun tree => tree).
 
   Definition rename dnum srcpath srcname dstpath dstname :=
-    retry_syscall (fun mscs => OptFS.rename fsxp dnum srcpath srcname dstpath dstname mscs)
+    retry_syscall (fun mscs => OptFS.rename (fsxp P) dnum srcpath srcname dstpath dstname mscs)
                   (fun tree => tree).
 
   Definition delete dnum name :=
-    retry_syscall (fun mscs => OptFS.delete fsxp dnum name mscs)
+    retry_syscall (fun mscs => OptFS.delete (fsxp P) dnum name mscs)
                   (fun tree => tree).
 
   (* wrap unverified syscalls *)
 
   Definition statfs :=
-    retry_syscall (fun mscs => OptFS.statfs fsxp mscs)
+    retry_syscall (fun mscs => OptFS.statfs (fsxp P) mscs)
                   (fun tree => tree).
 
   Definition mkdir dnum name :=
-    retry_syscall (fun mscs => OptFS.mkdir fsxp dnum name mscs)
+    retry_syscall (fun mscs => OptFS.mkdir (fsxp P) dnum name mscs)
                   (fun tree => tree).
 
   Definition file_get_sz inum :=
-    retry_syscall (fun mscs => OptFS.file_get_sz fsxp inum mscs)
+    retry_syscall (fun mscs => OptFS.file_get_sz (fsxp P) inum mscs)
                   (fun tree => tree).
 
   Definition file_set_sz inum sz :=
-    retry_syscall (fun mscs => OptFS.file_set_sz fsxp inum sz mscs)
+    retry_syscall (fun mscs => OptFS.file_set_sz (fsxp P) inum sz mscs)
                   (fun tree => tree).
 
   Definition readdir dnum :=
-    retry_syscall (fun mscs => OptFS.readdir fsxp dnum mscs)
+    retry_syscall (fun mscs => OptFS.readdir (fsxp P) dnum mscs)
                   (fun tree => tree).
 
   Definition tree_sync :=
-    retry_syscall (fun mscs => OptFS.tree_sync fsxp mscs)
+    retry_syscall (fun mscs => OptFS.tree_sync (fsxp P) mscs)
                   (fun tree => tree).
 
   Definition file_sync inum :=
-    retry_syscall (fun mscs => OptFS.file_sync fsxp inum mscs)
+    retry_syscall (fun mscs => OptFS.file_sync (fsxp P) inum mscs)
                   (fun tree => tree).
 
   Definition update_fblock inum off b :=
-    retry_syscall (fun mscs => OptFS.update_fblock fsxp inum off b mscs)
+    retry_syscall (fun mscs => OptFS.update_fblock (fsxp P) inum off b mscs)
                   (fun tree => tree).
 
   Definition mksock dnum name :=
-    retry_syscall (fun mscs => OptFS.mksock fsxp dnum name mscs)
+    retry_syscall (fun mscs => OptFS.mksock (fsxp P) dnum name mscs)
                   (fun tree => tree).
 
   Definition umount :=
-    retry_syscall (fun mscs => OptFS.umount fsxp mscs)
+    retry_syscall (fun mscs => OptFS.umount (fsxp P) mscs)
                   (fun tree => tree).
 
 End ConcurrentFS.
@@ -625,12 +396,13 @@ End ConcurrentFS.
 (* special identifier used for ghost variables, which are never allocated *)
 Definition absId : ident := 1000.
 
-Definition init (mscs: memstate) : cprog FsParams :=
+Definition init (fsxp: fs_xparams) (mscs: memstate) : cprog FsParams :=
   cacheId <- Alloc empty_cache;
     memstateId <- Alloc mscs;
     Ret {|
         cache:=cacheId;
         fsmem:=memstateId;
+        fsxp:=fsxp;
 
         vdisk:=absId;
         fstree:=absId;
