src/FSProtocol.v
@@ -1,0 +1,240 @@
+Require Import CCL.
+Require Import FSLayout.
+
+Require AsyncFS.
+(* imports for DirTreeRep.rep *)
+Import Log FSLayout Inode.INODE BFile.
+
+(* various other imports *)
+Export BFILE. (* importantly, exports memstate *)
+Import SuperBlock.
+Import GenSepN.
+Import Pred.
+
+Require Export HomeDirProtocol.
+Require Export OptimisticTranslator.
+
+Record FsParams :=
+  { cache: ident; (* : Cache *)
+    vdisk: ident; (* : Disk *)
+    fsmem: ident; (* : memsstate *)
+    fstree: ident; (* : dirtree *)
+    fshomedirs: ident; (* thread_homes *)
+    fsxp: fs_xparams;
+  }.
+
+Section FilesystemProtocol.
+
+  Variable P:FsParams.
+
+  Definition fs_rep vd hm mscs tree :=
+    exists ds ilist frees,
+      LOG.rep (FSLayout.FSXPLog (fsxp P)) (SB.rep (fsxp P))
+              (LOG.NoTxn ds) (MSLL mscs) hm (add_buffers vd) /\
+      (DirTreeRep.rep (fsxp P) Pred.emp tree ilist frees mscs)
+        (list2nmem (ds!!)).
+
+  Definition fs_invariant d hm tree (homedirs: thread_homes) : heappred :=
+    (fstree P |-> abs tree *
+     fshomedirs P |-> abs homedirs *
+     exists c vd mscs,
+       cache P |-> val c *
+       vdisk P |-> absMem vd *
+       [[ CacheRep d c vd ]] *
+       fsmem P |-> val mscs *
+       [[ fs_rep vd hm mscs tree ]])%pred.
+
+  Theorem fs_invariant_unfold : forall d hm tree homedirs h,
+      fs_invariant d hm tree homedirs h ->
+      exists c vd mscs,
+        (fstree P |-> abs tree * fshomedirs P |-> abs homedirs *
+         cache P |-> val c *
+         vdisk P |-> absMem vd *
+         fsmem P |-> val mscs)%pred h /\
+        CacheRep d c vd /\
+        fs_rep vd hm mscs tree.
+  Proof.
+    unfold fs_invariant; intros.
+    SepAuto.destruct_lifts.
+    descend; intuition eauto.
+  Qed.
+
+  Theorem fs_invariant_refold : forall tree homedirs d c vd hm mscs h,
+      (fstree P |-> abs tree * fshomedirs P |-> abs homedirs *
+       cache P |-> val c *
+       vdisk P |-> absMem vd *
+       fsmem P |-> val mscs)%pred h ->
+      CacheRep d c vd ->
+      fs_rep vd hm mscs tree ->
+      fs_invariant d hm tree homedirs h.
+  Proof.
+    unfold fs_invariant; intros.
+    SepAuto.pred_apply; SepAuto.cancel.
+  Qed.
+
+  Definition fs_guarantee tid (sigma sigma':Sigma) :=
+    exists tree tree' homedirs,
+      fs_invariant (Sigma.disk sigma) (Sigma.hm sigma) tree homedirs (Sigma.mem sigma) /\
+      fs_invariant (Sigma.disk sigma') (Sigma.hm sigma') tree' homedirs (Sigma.mem sigma') /\
+      homedir_guarantee tid homedirs tree tree' /\
+      Sigma.l sigma' = Sigma.l sigma.
+
+  Theorem fs_rely_same_fstree : forall tid sigma sigma' tree homedirs,
+      fs_invariant (Sigma.disk sigma) (Sigma.hm sigma) tree homedirs (Sigma.mem sigma) ->
+      fs_invariant (Sigma.disk sigma') (Sigma.hm sigma') tree homedirs (Sigma.mem sigma') ->
+      Sigma.l sigma' = Sigma.l sigma ->
+      Rely fs_guarantee tid sigma sigma'.
+  Proof.
+    intros.
+    constructor.
+    exists (S tid); intuition.
+    unfold fs_guarantee.
+    descend; intuition eauto.
+    reflexivity.
+  Qed.
+
+  Section InvariantUniqueness.
+
+    Ltac mem_eq m a v :=
+      match goal with
+      | [ H: context[ptsto a v] |- _ ] =>
+        let Hptsto := fresh in
+        assert ((exists F, F * a |-> v)%pred m) as Hptsto by
+              (SepAuto.pred_apply' H; SepAuto.cancel);
+        unfold exis in Hptsto; destruct Hptsto;
+        apply ptsto_valid' in Hptsto
+      end.
+
+    Lemma fs_invariant_tree_unique : forall d hm tree homedirs
+                                       d' hm' tree' homedirs' m,
+        fs_invariant d hm tree homedirs m ->
+        fs_invariant d' hm' tree' homedirs' m ->
+        tree = tree'.
+    Proof.
+      unfold fs_invariant; intros.
+      mem_eq m (fstree P) (abs tree).
+      mem_eq m (fstree P) (abs tree').
+      rewrite H1 in H2; inversion H2; inj_pair2.
+      auto.
+    Qed.
+
+    Lemma fs_invariant_homedirs_unique : forall d hm tree homedirs
+                                       d' hm' tree' homedirs' m,
+        fs_invariant d hm tree homedirs m ->
+        fs_invariant d' hm' tree' homedirs' m ->
+        homedirs = homedirs'.
+    Proof.
+      unfold fs_invariant; intros.
+      mem_eq m (fshomedirs P) (abs homedirs).
+      mem_eq m (fshomedirs P) (abs homedirs').
+      rewrite H1 in H2; inversion H2; inj_pair2.
+      auto.
+    Qed.
+
+  End InvariantUniqueness.
+
+  Ltac invariant_unique :=
+    repeat match goal with
+           | [ H: fs_invariant _ _ ?tree _ ?m,
+                  H': fs_invariant _ _ ?tree' _ ?m |- _ ] =>
+             first [ constr_eq tree tree'; fail 1 |
+                     assert (tree' = tree) by
+                         apply (fs_invariant_tree_unique H' H); subst ]
+           | [ H: fs_invariant _ _ _ ?homedirs ?m,
+                  H': fs_invariant _ _ _ ?homedirs' ?m |- _ ] =>
+             first [ constr_eq homedirs homedirs'; fail 1 |
+                     assert (homedirs' = homedirs) by
+                         apply (fs_invariant_homedirs_unique H' H); subst ]
+           end.
+
+  Theorem fs_rely_invariant : forall tid sigma sigma' tree homedirs,
+      fs_invariant (Sigma.disk sigma) (Sigma.hm sigma) tree homedirs (Sigma.mem sigma) ->
+      Rely fs_guarantee tid sigma sigma' ->
+      exists tree', fs_invariant (Sigma.disk sigma') (Sigma.hm sigma') tree' homedirs (Sigma.mem sigma').
+  Proof.
+    unfold fs_guarantee; intros.
+    generalize dependent tree.
+    induction H0; intros; repeat deex; eauto.
+    invariant_unique.
+    eauto.
+    edestruct IHclos_refl_trans1; eauto.
+  Qed.
+
+  Lemma fs_rely_invariant' : forall tid sigma sigma',
+      Rely fs_guarantee tid sigma sigma' ->
+      forall tree homedirs,
+        fs_invariant (Sigma.disk sigma) (Sigma.hm sigma) tree homedirs (Sigma.mem sigma) ->
+        exists tree',
+          fs_invariant (Sigma.disk sigma') (Sigma.hm sigma') tree' homedirs (Sigma.mem sigma').
+  Proof.
+    intros.
+    eapply fs_rely_invariant; eauto.
+  Qed.
+
+  Theorem fs_homedir_rely : forall tid sigma sigma' tree homedirs tree',
+      fs_invariant (Sigma.disk sigma) (Sigma.hm sigma) tree homedirs (Sigma.mem sigma) ->
+      Rely fs_guarantee tid sigma sigma' ->
+      fs_invariant (Sigma.disk sigma') (Sigma.hm sigma') tree' homedirs (Sigma.mem sigma') ->
+      homedir_rely tid homedirs tree tree'.
+  Proof.
+    unfold fs_guarantee; intros.
+    generalize dependent tree'.
+    generalize dependent tree.
+    apply Operators_Properties.clos_rt_rt1n in H0.
+    induction H0; intros; repeat deex; invariant_unique.
+    - reflexivity.
+    - match goal with
+      | [ H: homedir_guarantee _ _ _ _ |- _ ] =>
+        specialize (H _ ltac:(eauto))
+      end.
+      specialize (IHclos_refl_trans_1n _ ltac:(eauto) _ ltac:(eauto)).
+      unfold homedir_rely in *; congruence.
+  Qed.
+
+  Theorem fs_lock_rely : forall tid sigma sigma',
+      Rely fs_guarantee tid sigma sigma' ->
+      Sigma.l sigma' = Sigma.l sigma.
+  Proof.
+    unfold fs_guarantee; intros.
+    apply Operators_Properties.clos_rt_rt1n in H.
+    induction H; intros; repeat deex; congruence.
+  Qed.
+
+  Lemma fs_rely_preserves_subtree : forall tid sigma sigma' tree homedirs tree' path f,
+      find_subtree (homedirs tid ++ path) tree = Some f ->
+      fs_invariant (Sigma.disk sigma) (Sigma.hm sigma) tree homedirs (Sigma.mem sigma) ->
+      Rely fs_guarantee tid sigma sigma' ->
+      fs_invariant (Sigma.disk sigma') (Sigma.hm sigma') tree' homedirs (Sigma.mem sigma') ->
+      find_subtree (homedirs tid ++ path) tree' = Some f.
+  Proof.
+    intros.
+    eapply fs_homedir_rely in H1; eauto.
+    unfold homedir_rely in H1.
+    eapply find_subtree_app' in H; repeat deex.
+    erewrite find_subtree_app; eauto.
+    congruence.
+  Qed.
+
+  Theorem fs_guarantee_refl : forall tid sigma homedirs,
+      (exists tree, fs_invariant (Sigma.disk sigma) (Sigma.hm sigma) tree homedirs (Sigma.mem sigma)) ->
+      fs_guarantee tid sigma sigma.
+  Proof.
+    intros; deex.
+    unfold fs_guarantee; descend; intuition eauto.
+    reflexivity.
+  Qed.
+
+  Theorem fs_guarantee_trans : forall tid sigma sigma' sigma'',
+      fs_guarantee tid sigma sigma' ->
+      fs_guarantee tid sigma' sigma'' ->
+      fs_guarantee tid sigma sigma''.
+  Proof.
+    unfold fs_guarantee; intuition.
+    repeat deex; invariant_unique.
+
+    descend; intuition eauto.
+    etransitivity; eauto.
+    congruence.
+  Qed.
+
+End FilesystemProtocol.
